compose/Mod.v
@@ -50,13 +50,14 @@ Module Mod.
   Lemma get_modsem_projected_sk
         (md: t)
         skenv
+        (INCL: SkEnv.includes skenv (get_sk md (data md)))
     :
       <<PROJECTED: SkEnv.project_spec skenv ((md.(get_sk) md.(data)))
                                       ((md.(get_modsem) skenv) md.(data)).(ModSem.skenv)>>
   .
   Proof.
     erewrite <- get_modsem_skenv_spec.
-    eapply SkEnv.project_impl_spec.
+    eapply SkEnv.project_impl_spec; et.
   Qed.
 
   Definition sk (md: t): Sk.t := md.(get_sk) md.(data).
